Verity/Macro/Syntax.lean
@@ -22,6 +22,7 @@ syntax "revert " ident "(" sepBy(term, ",") ")" : doElem
 syntax "revertError " ident "(" sepBy(term, ",") ")" : doElem
 syntax "requireError " term:max ppSpace ident "(" sepBy(term, ",") ")" : doElem
 syntax "constructor " "(" sepBy(verityParam, ",") ")" " := " term : verityConstructor
+syntax "constructor " "(" sepBy(verityParam, ",") ")" " payable" " := " term : verityConstructor
 syntax "function " ident " (" sepBy(verityParam, ",") ")" " : " term " := " term : verityFunction
 
 syntax (name := verityContractCmd)
